remove := rfl antipattern

Computability/Constructions/EvalString.lean
@@ -55,26 +55,22 @@ def c_evalc :=
 
 @[simp] theorem c_evalc_ev: eval O c_evalc ⟪u, c, x⟫ = (evalc O u c x) := by
   unfold c_evalc
-  simp
-  simp [eval]
-  simp [Seq.seq]
-  simp [evalc]
+  simp [eval, Seq.seq, evalc]
   if h:(use O (n2c c) x).Dom then
-  simp [Part.Dom.bind h]
-  have hc1 : code_total O right := by exact right_total
-  have hc2 : code_total O (left.comp left) := by exact total_comp_of hc1 hc1
-  simp [c_if_le_te'_ev hc1 hc2]
-  simp [eval, Seq.seq]
+    simp [Part.Dom.bind h]
+    have hc1 : code_total O right := by exact right_total
+    have hc2 : code_total O (left.comp left) := by exact total_comp_of hc1 hc1
+    simp [c_if_le_te'_ev hc1 hc2]
+    simp [eval, Seq.seq]
   else
-  simp [Part.eq_none_iff'.mpr h]
+    simp [Part.eq_none_iff'.mpr h]
 
 end Computability.Code
--- theorem Nat.PrimrecIn.evalc:Nat.PrimrecIn O evalc := by ...
--- theorem Nat.Primrec.evalc:Nat.Primrec Nat.evalc := by ...
 end evalc
 
 section evals
 namespace Computability.Code
+section c_evalo
 def c_evalo :=
   let o := left
   let c := left.comp right
@@ -84,8 +80,9 @@ theorem c_evalo_ev (ho:code_total O o) : eval O c_evalo ⟪o, c, x⟫ = eval (λ
   simp [c_evalo]
   simp [eval,Seq.seq]
   rw [@eval_replace_oracle_prop O o c ho]
+end c_evalo
 
-
+section c_evals_oracle
 def c_evals_oracle (o:Code):= c_sg.comp $ c_list_getD.comp₃ (c_const o) c_id (c_const whatever)
 @[cp] theorem c_evals_oracle_prim : code_prim (c_evals_oracle o) := by unfold c_evals_oracle; apply_cp
 theorem c_evals_oracle_evp : evalp O (c_evals_oracle o) =
@@ -104,7 +101,9 @@ theorem c_evals_oracle_ev : eval O (c_evals_oracle o) =
 := by
   simp [← evalp_eq_eval c_evals_oracle_prim]
   simp [c_evals_oracle_evp]
+end c_evals_oracle
 
+section c_comp₂
 def c_comp₂ :=
   let a := left
   let b := left.comp right
@@ -114,6 +113,8 @@ def c_comp₂ :=
 @[simp] theorem c_comp₂_evp : evalp O c_comp₂ ⟪a,b,c⟫ = c2n (comp₂ a b c) := by
   simp [c_comp₂]; rfl
 @[simp] theorem c_comp₂_ev:eval O c_comp₂ ⟪a,b,c⟫ = c2n (comp₂ a b c) := by rw [← evalp_eq_eval c_comp₂_prim]; simp
+end c_comp₂
+section c_comp₃
 def c_comp₃ :=
   let a := left.comp left
   let b := left.comp right
@@ -124,36 +125,29 @@ def c_comp₃ :=
 @[simp] theorem c_comp₃_evp : evalp O c_comp₃ ⟪⟪a,b⟫,⟪c,d⟫⟫ = c2n (comp₃ a b c d) := by
   simp [c_comp₃]; rfl
 @[simp] theorem c_comp₃_ev:eval O c_comp₃ ⟪⟪a,b⟫,⟪c,d⟫⟫ = c2n (comp₃ a b c d) := by rw [← evalp_eq_eval c_comp₃_prim]; simp
+end c_comp₃
 
+section c_c_evals_oracle
 def c_c_evals_oracle := c_comp.comp₂ (c_const c_sg) (c_comp₃.comp₄ (c_const c_list_getD) (c_c_const.comp left) (c_const c_id) (c_const $ c_const whatever))
 @[cp] def c_c_evals_oracle_prim : code_prim c_c_evals_oracle := by unfold c_c_evals_oracle; apply_cp
 @[simp] theorem c_c_evals_oracle_evp : evalp O c_c_evals_oracle ⟪o,c,x⟫ =
 c2n (c_evals_oracle o) := by simp [c_c_evals_oracle, c_evals_oracle]
-
 theorem c_c_evals_oracle_ev : eval O c_c_evals_oracle ⟪o,c,x⟫ = c2n (c_evals_oracle o) := by simp [← evalp_eq_eval c_c_evals_oracle_prim]
+end c_c_evals_oracle
 
+section c_evals
 def c_evals_code := c_evalc.comp₂ (c_list_length.comp left) right
-
-theorem c_evals_code_ev : eval O c_evals_code ⟪o,c,x⟫ =
-evalc O (n2l o).length c x
-:= by
-
+theorem c_evals_code_ev : eval O c_evals_code ⟪o,c,x⟫ = evalc O (n2l o).length c x := by
   simp [c_evals_code]
   simp [eval, Seq.seq]
-
-def c_evals :=
-  c_evalo.comp₃
+def c_evals := c_evalo.comp₃
   c_c_evals_oracle
   (c_const c_evals_code)
   c_id
-
 @[simp] theorem c_evals_ev: eval O c_evals ⟪o,c,x⟫ = (evals (n2l o) c x) := by
   unfold evals
   unfold c_evals
-  simp
-
   simp [Seq.seq]
-
   have t1 : code_total O c_c_evals_oracle := prim_total c_c_evals_oracle_prim
   have : code_total O ((eval O c_c_evals_oracle ⟪o,c,x⟫).get (t1 ⟪o,c,x⟫)) := by
     simp [c_c_evals_oracle_ev]
@@ -166,9 +160,6 @@ def c_evals :=
   simp [c_c_evals_oracle_ev]
   simp [c_evals_oracle_ev]
   simp [c_evals_code_ev]
-
-
+end c_evals
 end Computability.Code
--- theorem Nat.PrimrecIn.evals:Nat.PrimrecIn O evals := by ...
--- theorem Nat.Primrec.evals:Nat.Primrec Nat.evals := by ...
 end evals
